show the that Prop monad has mfix

theories/MFixITree.v
@@ -1,7 +1,9 @@
 Require Import ITree.ITree.
+Require Import ITree.Fix.
 Require Import ExtLib.Structures.Monads.
 
 Import MonadNotation.
+
 
 Section M.
   (* The effects interface *)
@@ -10,9 +12,11 @@ Section M.
   Variable M : Type -> Type.
   Variable m : Monad M.
 
+  (*
   (* Monads are functors *)
   Variable fmap_M : forall A B, (A -> B) -> M A -> M B.
-
+  *)
+  (*
   (* We can write [join] in terms of [bind] *)
   Definition join {X} (e : M (M X)) : M X :=
     bind e (fun y => y).
@@ -23,7 +27,14 @@ Section M.
     fun (x:A) =>
       bind f (fun g => ret (g x)).
 
+*)
+  (* A monadic "handler" for some effects E is just a mapping from
+     the actions to monadic computations that return values of the 
+     right type. *)
+  Variable handler : forall {X} (e:IO X), M X.
 
+  
+(*
   (* Note: the other direction is BOGUS -- we can't "run" the effects 
      of a function's body _before_ returning the function.  *)
   (* Definition coerce2 {A B} (f : A -> M B) : M (A -> B) := BOGUS *)
@@ -43,10 +54,6 @@ Section M.
      unlike the Haskell presentation. *)
 
   
-  (* A monadic "handler" for some effects E is just a mapping from
-     the actions to monadic computations that return values of the 
-     right type. *)
-  Variable handler : forall {X} (e:IO X), M X.
   
 
   (* We can interpret an itree into any monad that supports mfix as follows: *)
@@ -64,81 +71,66 @@ Section M.
 
           )) t).
 
-
+*)
   (* Version 2: Correct version of MFix -------------------------------------- *)
-  Variable mfix'' : forall A B, ((A -> M B) -> (A -> M B)) -> A -> M B.
+
+  Definition mfix_weak := forall A B, ((A -> M B) -> (A -> M B)) -> A -> M B.
+
+  
+  Definition mfix_type := forall A B, (forall N `{Monad N} (inc:forall A, M A -> N A), ((A -> N B) -> (A -> N B))) -> A -> M B.
+  Variable mfix_parametric : mfix_type.
 
   Definition run'' {X} (t : itree IO X) : M X :=
-            mfix'' (itree IO X) X
-                   ( fun (f : (itree IO X -> M X)) =>
+            mfix_parametric (itree IO X) X 
+                   ( fun N _ inc (f : (itree IO X -> N X)) =>
                        (fun (u : itree IO X) =>
                           match u with
                           | Ret x => ret x
                           | Tau w => f w
                           | Vis e k =>
-                            bind (handler _ e) (fun a => f (k a))
+                            bind (inc _ (handler _ e)) (fun a => f (k a))
                           end)
                      ) t.
-  
-
-(* below here is probably junk ---------------------------------------------- *)
-
-  
-  (* Note, can weaken the requirements on mfix for the purposes of our
-  development because we only need to use mfix at a funnction type.  That is, we
-  could specialize things to: *)
-  Variable mfix' : forall A B, ((A -> B) -> M (A -> B)) -> M (A -> B).
-
-  (* It might be "easier" to implement a monad that support mfix' than one that supports general mfix. *)
-  
-  Definition run' {X} (t : itree IO X) : M X :=
-    join ((coerce1 (mfix' (itree IO X) (M X)
-                         ( fun (f : (itree IO X -> M X)) =>
-                             (ret (fun (u : itree IO X) =>
-                                     match u with
-                                     | Ret x => ret x
-                                     | Tau w => f w
-                                     | Vis e k =>
-                                       bind (handler _ e) (fun a => f (k a))
-                                     end)
-                         )) 
-
-          )) t).
-
-
-
-
-  
-  
-(*
-  CoFixpoint handle {X} (t : itree IO X) : itree MIO X :=
-    match t with
-    | Ret v => Ret v
-    | Tau u => Tau (handle u)
-    | Vis e k => 
-      Vis (handler e)
-          (fun (m : M (E_reaction io)) => _)
-    end.
-*)
-(*  
-  CoInductive run {X} : itree IO X -> M X -> Prop :=
-  | run_ret : forall v, run (Ret v) (ret v)
-  | run_tau : forall u r, run u r -> run (Tau u) r
-  | run_vis : forall e k r,
-      exists t, run (fmap_M _ _ k (handler e)) = t.
-      run (Vis e k) (bind r k)
-  
-
-  CoInductive run {X} : itree IO X -> M (itree IO X) -> Prop :=
-  | run_ret : forall v, run (Ret v) (ret (Ret v))
-  | run_tau : forall u r, run u r -> run (Tau u) (bind r (fun v => ret (Tau v)))
-  | run_vis : forall e k r,
-      run (handler e) r ->
-      run (Vis e k) (bind r k)
- *)
 
 End M.
 
+Require Import Paco.paco.
 
-    
+Check paco2.
+
+Section P.
   
+  Definition mfix_P {a b:Type} (f : ((a -> b -> Prop) -> (a -> b -> Prop))) : a -> b -> Prop :=
+    @paco2 a (fun _ => b) f bot2.
+
+  Lemma mfix_law1 : forall (a b : Type) f (x:a) (y:b), (@monotone2 a (fun _ => b) f) -> (mfix_P f x y) -> f (mfix_P f) x y.
+  Proof.
+    intros a b f x y Hm H. 
+    punfold H. unfold mfix_P. unfold upaco2 in H. unfold monotone2 in Hm.
+    eapply Hm. apply H.
+    intros. inversion PR. exact H0. inversion H0.
+  Qed.
+
+  Lemma mfix_law2 : forall (a b : Type) f (x:a) (y:b), (@monotone2 a (fun _ => b) f) -> f (mfix_P f) x y -> (mfix_P f x y).
+  Proof.
+    intros a b f x y Hm H.
+    unfold mfix_P.
+    pfold. unfold mfix_P in H. unfold monotone2 in Hm. eapply Hm. apply H.
+    intros x0 x1 PR.
+    left. exact PR.
+  Qed.
+
+End P.
+    
+
+Variable E: Type -> Type.
+
+Check Fix.FixImpl.mfix.
+Locate MonadFix.
+Set Printing Universes.
+Print mfix_type.
+Print Monad_itree.
+Definition mfix_itree : mfix_type (itree E) :=
+  fun A B f => Fix.FixImpl.mfix (fun _ => B) (fun E' inc rec => f (itree E') (Monad_itree) inc rec).
+
+      
